Prove top-level file_get_attr syscall theorem

src/ConcurrentFS.v
@@ -1,4 +1,5 @@
 Require Import CCL.
+Require Import Hashmap.
 Require Import OptimisticTranslator OptimisticFS.
 
 Require AsyncFS.
@@ -40,27 +41,56 @@ Section ConcurrentFS.
   Definition get_homedirs (sigma: Sigma St) :=
     homedirs (cache_other_s (Sigma.s sigma)).
 
-  Definition fs_invariant wb (sigma: Sigma St) :=
-    let tree := get_fstree sigma in
-    let mscs := get_fsmem (Sigma.mem sigma) in
-    CacheRep wb sigma /\
+  Definition fs_rep d tree mscs hm :=
     exists ds ilist frees,
       LOG.rep (FSLayout.FSXPLog fsxp) (SB.rep fsxp)
-              (LOG.NoTxn ds) (MSLL mscs) (Sigma.hm sigma)
-              (seq_disk sigma) /\
+              (LOG.NoTxn ds) (MSLL mscs) hm d /\
       (DirTreeRep.rep fsxp Pred.emp tree ilist frees)
         (list2nmem (ds!!)).
 
-  Definition fs_guarantee' wb' tid (sigma sigma':Sigma St) :=
-    fs_invariant empty_writebuffer sigma /\
-    fs_invariant wb' sigma' /\
+  Definition fs_invariant (sigma: Sigma St) :=
+    let tree := get_fstree sigma in
+    let mscs := get_fsmem (Sigma.mem sigma) in
+    CacheRep empty_writebuffer sigma /\
+    fs_rep (seq_disk sigma) tree mscs (Sigma.hm sigma).
+
+  Definition fs_guarantee tid (sigma sigma':Sigma St) :=
+    fs_invariant sigma /\
+    fs_invariant sigma' /\
     let tree := get_fstree sigma in
     let tree' := get_fstree sigma' in
     homedir_guarantee tid (get_homedirs sigma) tree tree' /\
     get_homedirs sigma' = get_homedirs sigma.
 
-  Definition fs_guarantee :=
-    fs_guarantee' empty_writebuffer.
+  Theorem fs_rely_same_fstree : forall tid sigma sigma',
+      fs_invariant sigma ->
+      fs_invariant sigma' ->
+      get_fstree sigma' = get_fstree sigma ->
+      get_homedirs sigma' = get_homedirs sigma ->
+      Rely fs_guarantee tid sigma sigma'.
+  Proof.
+    unfold fs_guarantee; intros.
+    constructor.
+    exists (S tid); intuition.
+    rewrite H1.
+    apply homedir_guar_preorder.
+  Qed.
+
+  Theorem fs_guarantee_refl : forall tid sigma,
+      fs_invariant sigma ->
+      fs_guarantee tid sigma sigma.
+  Proof.
+    unfold fs_guarantee; intuition.
+  Qed.
+
+  Theorem fs_rely_invariant : forall tid sigma sigma',
+      fs_invariant sigma ->
+      Rely fs_guarantee tid sigma sigma' ->
+      fs_invariant sigma'.
+  Proof.
+    induction 2; intros; repeat deex; intuition eauto.
+    unfold fs_guarantee in *; intuition.
+  Qed.
 
   (* TODO: eventually abstract away protocol *)
 
@@ -125,97 +155,154 @@ Section ConcurrentFS.
            | _ => progress subst
            end.
 
-  Section GetAttrCleanSpec.
-
-    Hint Extern 0 {{ OptFS.file_get_attr _ _ _ _ _; _ }} => apply OptFS.file_get_attr_ok : prog.
-
-    Ltac descend :=
-      repeat match goal with
-             | [ |- exists _, _ ] => eexists
-             end.
-
-    Lemma fstree_locally_modified : forall sigma sigma',
-        locally_modified sigma sigma' ->
-        get_fstree sigma' = get_fstree sigma.
-    Proof.
-      unfold get_fstree, locally_modified.
-      destruct sigma, sigma'; simpl; intuition congruence.
-    Qed.
-
-    Theorem file_get_attr1_ok : forall inum tid mscs,
-        cprog_spec fs_guarantee tid
-                   (fun '(pathname, f) '(sigma_i, sigma) =>
-                      {| precondition :=
-                           fs_guarantee tid sigma_i sigma /\
-                           mscs = get_fsmem (Sigma.mem sigma) /\
-                           let tree := get_fstree sigma in
-                           find_subtree pathname tree = Some (TreeFile inum f);
-                         postcondition :=
-                           fun '(sigma_i', sigma') '(r, wb') =>
-                             get_fstree sigma' = get_fstree sigma /\
-                             match r with
-                             | Success (mscs', (r, _)) =>
-                               r = BFILE.BFAttr f /\
-                               fs_guarantee' wb' tid sigma_i'
-                                             (Sigma.set_mem sigma' (set_fsmem (Sigma.mem sigma') mscs'))
-                             | Failed =>
-                               (* need to promise committed disk doesn't change *)
-                               locally_modified sigma sigma' /\
-                               CacheRep wb' sigma'
-                             end
-                      |}) (OptFS.file_get_attr _ fsxp inum mscs empty_writebuffer).
-    Proof.
-      intros.
-      step.
-
-      unfold OptFS.framed_spec, translate_spec; simpl.
-      repeat apply exists_tuple; simpl.
-      unfold fs_guarantee, fs_guarantee', fs_invariant in *; intuition;
-        repeat deex.
-
-      descend; intuition eauto.
-      SepAuto.pred_apply; SepAuto.cancel; eauto.
-
-      step.
-
-      intuition eauto.
-      apply fstree_locally_modified; auto.
-
-      destruct a.
-      - (* translated code returned success *)
-        destruct v as (mscs' & (attr & u)); destruct u.
-        split_lift_prop; auto.
-        intuition eauto.
-
-        destruct sigma, sigma'; simpl in *; eauto.
-
-        fold St in *.
-        unfold locally_modified, get_fstree in *.
-        destruct sigma, sigma'; simpl in *; eauto.
-        exists ds, ilist, frees.
-        intuition eauto.
-        congruence.
-
-        unfold locally_modified, get_fstree in *.
-        destruct sigma, sigma' in *; simpl in *; intuition eauto.
-        etransitivity; eauto.
-        match goal with
-        | [ |- homedir_guarantee _ _ ?tree ?tree' ] =>
-          replace tree' with tree by congruence
-        end; reflexivity.
-
-        unfold get_homedirs, set_fsmem, get_fstree, locally_modified in *.
-        destruct sigma_i, sigma, sigma' in *; simpl in *; intuition.
-        congruence.
-      - intuition eauto.
-    Qed.
-
-  End GetAttrCleanSpec.
-
-  Hint Extern 0 {{ OptFS.file_get_attr _ _ _ _ _; _ }} => apply file_get_attr1_ok : prog.
-
   Hint Extern 0 {{ CacheCommit _; _ }} => apply CacheCommit_ok : prog.
   Hint Extern 0 {{ CacheAbort; _ }} => apply CacheAbort_ok : prog.
+
+  Lemma locally_modified_fstree : forall sigma sigma',
+      locally_modified sigma sigma' ->
+      get_fstree sigma' = get_fstree sigma.
+  Proof.
+    unfold get_fstree, locally_modified; intros.
+    destruct sigma, sigma'; simpl in *; intuition congruence.
+  Qed.
+
+  Lemma locally_modified_fsmem : forall sigma sigma',
+      locally_modified sigma sigma' ->
+      get_fsmem (Sigma.mem sigma') = get_fsmem (Sigma.mem sigma).
+  Proof.
+    unfold get_fsmem, locally_modified; intros.
+    destruct sigma, sigma'; simpl in *; intuition congruence.
+  Qed.
+
+  Lemma locally_modified_homedirs : forall sigma sigma',
+      locally_modified sigma sigma' ->
+      get_homedirs sigma' = get_homedirs sigma.
+  Proof.
+    unfold get_homedirs, locally_modified; intros.
+    destruct sigma, sigma'; simpl in *; intuition congruence.
+  Qed.
+
+  Ltac learning :=
+    repeat match goal with
+           | [ H: locally_modified _ _ |- _ ] =>
+             learn that (locally_modified_fstree H)
+           | [ H: locally_modified _ _ |- _ ] =>
+             learn that (locally_modified_fsmem H)
+           | [ H: locally_modified _ _ |- _ ] =>
+             learn that (locally_modified_homedirs H)
+           | [ H: CacheRep empty_writebuffer _ |- _ ] =>
+             learn that (CacheRep_empty H)
+           end.
+
+  Lemma upd_fstree_id : forall up sigma,
+      (forall tree, up tree = tree) ->
+      upd_fstree up sigma = sigma.
+  Proof.
+    unfold upd_fstree.
+    destruct sigma, cache_other_s; simpl; intros.
+    rewrite H; auto.
+  Qed.
+
+  Lemma get_set_fsmem : forall m mscs,
+      get_fsmem (set_fsmem m mscs) = mscs.
+  Proof.
+    reflexivity.
+  Qed.
+
+  Lemma seq_disk_set_fsmem : forall d m mscs s hm,
+      seq_disk (state d (set_fsmem m mscs) s hm) = seq_disk (state d m s hm).
+  Proof.
+    reflexivity.
+  Qed.
+
+  Lemma get_fstree_set_fsmem : forall d m mscs s hm,
+      get_fstree (state d (set_fsmem m mscs) s hm) = get_fstree (state d m s hm).
+  Proof.
+    reflexivity.
+  Qed.
+
+  Hint Rewrite upd_fstree_id using solve [ auto ] : get_set.
+  Hint Rewrite get_set_fsmem seq_disk_set_fsmem get_fstree_set_fsmem : get_set.
+
+  Ltac simplify :=
+    repeat match goal with
+           | [ H: get_fstree _ = get_fstree _ |- _ ] =>
+             rewrite H in *
+           | _ => progress autorewrite with get_set
+           | _ => progress simpl
+           end.
+
+  Theorem opt_file_get_attr_ok : forall inum mscs wb tid,
+      cprog_spec fs_guarantee tid
+                 (fun '(pathname, f) '(sigma_i, sigma) =>
+                    {| precondition :=
+                         let tree := get_fstree sigma in
+                         mscs = get_fsmem (Sigma.mem sigma) /\
+                         CacheRep wb sigma /\
+                         fs_rep (seq_disk sigma) tree mscs (Sigma.hm sigma) /\
+                         find_subtree pathname tree = Some (TreeFile inum f);
+                       postcondition :=
+                         fun '(sigma_i', sigma') '(r, wb') =>
+                           CacheRep wb' sigma' /\
+                           locally_modified sigma sigma' /\
+                           hashmap_le (Sigma.hm sigma) (Sigma.hm sigma') /\
+                           vdisk_committed (Sigma.s sigma') = vdisk_committed (Sigma.s sigma) /\
+                           match r with
+                           | Success (mscs', (r, _)) =>
+                             r = BFILE.BFAttr f /\
+                             fs_rep (seq_disk sigma') (get_fstree sigma) mscs' (Sigma.hm sigma')
+                           | Failed =>
+                             fs_rep (seq_disk sigma) (get_fstree sigma) mscs (Sigma.hm sigma') /\
+                             get_fsmem (Sigma.mem sigma') = get_fsmem (Sigma.mem sigma)
+                           end /\
+                           sigma_i' = sigma_i; |})
+                 (OptFS.file_get_attr _ fsxp inum mscs wb).
+  Proof.
+    prestep; step_using ltac:(apply OptFS.file_get_attr_ok).
+
+    unfold fs_rep in *; intuition eauto; repeat deex.
+    destruct ds.
+    destruct sigma; simpl in *.
+    repeat apply exists_tuple; descend; simpl; intuition eauto.
+
+    SepAuto.pred_apply; SepAuto.cancel.
+    eauto.
+
+    step.
+    intuition eauto.
+    destruct a as [(mscs & (attr & u)) | ]; split_lift_prop; intuition eauto.
+
+    descend; intuition eauto.
+    eapply LOG.rep_hashmap_subset; eauto.
+
+    learning; congruence.
+  Qed.
+
+  Hint Extern 0 {{ OptFS.file_get_attr _ _ _ _ _; _ }} => apply opt_file_get_attr_ok : prog.
+
+  Lemma and_copy : forall (P Q:Prop),
+      P ->
+      (P -> Q) ->
+      P /\ Q.
+  Proof.
+    eauto.
+  Qed.
+
+  Lemma rely_file_preserved : forall sigma sigma' tid pathname f,
+      find_subtree (get_homedirs sigma tid ++ pathname) (get_fstree sigma) = Some f ->
+      Rely fs_guarantee tid sigma sigma' ->
+      find_subtree (get_homedirs sigma' tid ++ pathname) (get_fstree sigma') = Some f.
+  Proof.
+    unfold Rely, fs_guarantee; intros.
+    induction H0; intuition; repeat deex.
+    unfold homedir_guarantee in H3.
+    specialize (H3 _ ltac:(eauto)).
+    unfold homedir_rely in H3.
+
+    apply find_subtree_app' in H; deex; intuition.
+    erewrite find_subtree_app; eauto.
+    congruence.
+  Qed.
 
   Theorem file_get_attr_ok : forall inum tid,
       cprog_spec fs_guarantee tid
@@ -223,54 +310,145 @@ Section ConcurrentFS.
                     {| precondition :=
                          fs_guarantee tid sigma_i sigma /\
                          let tree := get_fstree sigma in
-                         find_subtree pathname tree = Some (TreeFile inum f);
+                         find_subtree (get_homedirs sigma tid ++ pathname) tree = Some (TreeFile inum f);
                        postcondition :=
                          fun '(sigma_i', sigma') r =>
                            Rely fs_guarantee tid sigma sigma' /\
-                           get_fstree sigma' = get_fstree sigma /\
                            match r with
                            | Success (r, _) => r = BFILE.BFAttr f
                            | Failed => True
-                           end
+                           end /\
+                           fs_guarantee tid sigma_i' sigma'
                     |}) (file_get_attr inum).
   Proof.
     unfold file_get_attr, retry_syscall; intros.
 
-    eapply retry_spec'; induction n; simpl.
+    eapply retry_spec' with (Failed).
+    simpl.
+    induction n; simpl.
+    - step.
+      step.
+      intuition eauto.
+      constructor.
+      exists (S tid); intuition.
+      unfold fs_guarantee in *; simpl in *; intuition eauto.
+      apply homedir_guar_preorder.
     - step.
       step.
 
-      apply exists_tuple; do 2 eexists; simpl; intuition eauto.
+      match goal with
+      | [ H: fs_guarantee _ _ _ |- _ ] =>
+        unfold fs_guarantee, fs_invariant in H; intuition; repeat deex
+      end.
+
+      repeat apply exists_tuple; descend; simpl; intuition eauto.
 
       destruct a as [(mscs & (attr & u)) | ].
       + step.
 
         intuition eauto.
 
-        unfold fs_guarantee', fs_invariant in H5; intuition eauto.
-        destruct sigma'; simpl in *; eauto.
-
         hoare.
+        destruct (guard r); repeat deex.
+        step.
+
+        match goal with
+        | [ H: Success _ = Success _ |- _ ] =>
+          inversion H; subst; clear H
+        end.
+        split_lift_prop.
+        learning.
+
+        destruct sigma, sigma0, sigma'; simpl in *; simplify.
         intuition eauto.
-        admit. (* rely holds *)
-        admit. (* fstree unchanged *)
+
+        eapply fs_rely_same_fstree; unfold fs_invariant; intuition eauto.
+        simplify; subst; eauto.
+
+        unfold seq_disk, get_fstree in *; simpl in *.
+        congruence.
+
+        unfold get_homedirs in *; simpl in *; congruence.
+
+        unfold fs_guarantee; intuition eauto.
+        unfold fs_guarantee, fs_invariant in *; intuition eauto.
+        unfold fs_guarantee, fs_invariant in *; simplify; intuition eauto.
+        unfold seq_disk, get_fstree in *; simpl in *; congruence.
+
+        simplify.
+        unfold get_homedirs, get_fstree in *; simpl in *.
+        etransitivity; eauto.
+        congruence.
+
+        unfold get_homedirs in *; simpl in *; congruence.
+
+        subst.
+        step.
+        congruence.
       + hoare.
+
+        apply and_copy.
+
+        unfold fs_guarantee; intuition eauto.
+        unfold fs_invariant in *; intuition eauto.
+        unfold fs_invariant, fs_guarantee in *; intuition eauto.
+
+        learning; simplify.
+        destruct sigma_i, sigma, sigma', sigma0 in *; simpl in *; subst; eauto.
+        unfold seq_disk in *; simpl in *; eauto.
+        congruence.
+
+        learning; simplify.
+        etransitivity; eauto.
+        match goal with
+        | [ |- homedir_guarantee _ _ ?tree ?tree' ] =>
+          replace tree with tree' by congruence; reflexivity
+        end.
+
+        learning; simplify.
+        unfold get_homedirs in *; simpl in *.
+        congruence.
+
+        step.
+        repeat apply exists_tuple; descend; simpl; intuition eauto.
+
+        eapply fs_guarantee_refl.
+        match goal with
+        | [ H: Rely fs_guarantee _ _ _ |- _ ] =>
+          eapply fs_rely_invariant in H; eauto
+        end.
+        unfold fs_guarantee in *; intuition eauto.
+
+        learning.
+        match goal with
+        | [ H: find_subtree (get_homedirs ?sigma ?tid ++ _) ?tree = Some _,
+               H': Rely fs_guarantee ?tid ?sigma' _ |- _ ] =>
+          replace (get_homedirs sigma tid) with (get_homedirs sigma' tid) in H by congruence;
+            replace tree with (get_fstree sigma') in H by congruence
+        end.
+
+        eapply rely_file_preserved; eauto.
+
+        step.
         intuition eauto.
-        admit.
 
-        hoare.
-        intuition eauto.
-        unfold Rely.
-        eapply Relation_Operators.rt_trans; eauto.
-        fold (Rely fs_guarantee tid sigma sigma0).
-        admit.
+        Lemma rely_trans : forall St (G: Protocol St) tid sigma sigma' sigma'',
+            Rely G tid sigma sigma' ->
+            Rely G tid sigma' sigma'' ->
+            Rely G tid sigma sigma''.
+        Proof.
+          unfold Rely; intros.
+          eapply Relation_Operators.rt_trans; eauto.
+        Qed.
 
-        admit.
-    - hoare.
-      apply exists_tuple; do 2 eexists; simpl; intuition eauto.
-
-      destruct a as [(mscs & (attr & u)) | ].
-  Abort.
+        eapply rely_trans; eauto.
+        eapply rely_trans; eauto.
+        eapply fs_rely_same_fstree; eauto.
+        unfold fs_invariant; intuition eauto.
+        unfold fs_guarantee in *; intuition eauto.
+        learning; congruence.
+        learning; congruence.
+  Qed.
 
 End ConcurrentFS.
 
